check_inplace_hash file.3d=file.h

src/3d/ocaml/Batch.ml
@@ -377,6 +377,20 @@ let hashed_files
       else None;
   }
 
+let check_inplace_hash
+  file_3d_file_c
+=
+  match String.split_on_char '=' file_3d_file_c with
+  | [file_3d; file_c] ->
+    if Hashing.check_inplace_hashes file_3d (Hashing.OneHash file_c)
+    then begin
+      print_endline (Printf.sprintf "EverParse check_inplace_hash succeeded on %s" file_3d)
+    end else
+      failwith (Printf.sprintf "EverParse check_inplace_hash failed on %s" file_3d)
+  | _ -> failwith "check_inplace_hash: expected file.3d=file.h"
+
+let check_inplace_hashes = List.iter check_inplace_hash
+
 let check_hashes
   (ch: check_hashes_t)
   (out_dir: string)
@@ -385,7 +399,7 @@ let check_hashes
   let c = hashed_files out_dir modul in
   match ch with
   | InplaceHashes ->
-    Hashing.check_inplace_hashes file c
+    Hashing.check_inplace_hashes file (Hashing.AllHashes c)
   | _ ->
     let json = filename_concat out_dir (Printf.sprintf "%s.json" modul) in
     Hashing.check_hash file None json && (
